review feedback
Signed-off-by: Shaobo He <shaobohe@amazon.com>

cedar-lean/Cedar/Thm/Validation/Typechecker/Types.lean
@@ -84,10 +84,10 @@ def InstanceOfEntityTags (data : EntityData) (entry : EntitySchemaEntry) : Prop 
   | .some tty => ∀ v ∈ data.tags.values, InstanceOfType v tty
   | .none     => data.tags = Map.empty
 
-def IsValidEntityUID (entry: EntitySchemaEntry) (eid: String) : Prop :=
+def IsValidEntityEID (entry: EntitySchemaEntry) (eid: String) : Prop :=
   match entry with
   | .standard _ => True
-  | .enum eids => ∃ eid₁, eid₁ ∈ eids ∧ eid₁ = eid
+  | .enum eids => eid ∈ eids
 
 /--
 For every entity in the store,
@@ -100,7 +100,7 @@ For every entity in the store,
 def InstanceOfEntitySchema (entities : Entities) (ets: EntitySchema) : Prop :=
   ∀ uid data, entities.find? uid = some data →
     ∃ entry, ets.find? uid.ty = some entry ∧
-      IsValidEntityUID entry uid.eid ∧
+      IsValidEntityEID entry uid.eid ∧
       InstanceOfType data.attrs (.record entry.attrs) ∧
       (∀ ancestor, ancestor ∈ data.ancestors → ancestor.ty ∈ entry.ancestors) ∧
       InstanceOfEntityTags data entry
